src/tls/Extensions.fst
@@ -14,8 +14,6 @@ open Platform.Error
 open TLSError
 open TLSConstants
 
-module TI = TLSInfo
-
 (*************************************************
  Define extension. 
  *************************************************)
@@ -32,55 +30,44 @@ noeq type psk =
 type psk_kex =
   | PSK_KE 
   | PSK_DHE_KE 
+
 type client_psk_kexes = l:list psk_kex 
   { l = [PSK_KE] \/ l = [PSK_DHE_KE] \/ l = [PSK_KE; PSK_DHE_KE] \/ l = [PSK_DHE_KE; PSK_KE] }
 
 // The length reflects the RFC format constraint <2..254> 
-type protocol_versions = l: list TLSConstants.protocolVersion {List.Tot.length l >= 1 /\ List.Tot.length l <= 127}
+type protocol_versions =
+  l:list protocolVersion {0 < List.Tot.length l /\ List.Tot.length l < 128}
+
+type earlyDataIndication = option UInt32.t // Only Some for NewSessionTicket
 
 (** RFC 4.2 'Extension' Table's type definition. *)
-noeq type preEarlyDataIndication : Type0 =
-  { ped_configuration_id: configurationId;
-    ped_cipher_suite:valid_cipher_suite;
-    ped_extensions:list extension;
-    ped_context:b:bytes{length b < 256};
-    //ped_early_data_type:earlyDataType;
-    }
-and earlyDataIndication =
-  | ClientEarlyDataIndication of preEarlyDataIndication
-  | ServerEarlyDataIndication
-(* SI: we currently only define Mandatory-to-Implement Extensions 
-   as listed in the RFC's Section 8.2. Labels in the variants below are: 
-     M  - "MUST implement"
-     AF - "MUST ... when offering applicable features" *)
-and extension =
-  | E_server_name of list TI.serverName (* M, AF *) (* RFC 6066 *)
-(*| E_max_fragment_length
-  | E_status_request *)
+noeq 
+type extension =
+  | E_server_name of list serverName (* M, AF *) (* RFC 6066 *)
   | E_supported_groups of list namedGroup (* M, AF *) (* RFC 7919 *)  
   | E_signature_algorithms of (list sigHashAlg) (* M, AF *) (* RFC 5246 *)
-(*| E_use_srtp 
+  | E_key_share of CommonDH.keyShare (* M, AF *)
+  | E_pre_shared_key of (list psk) (* M, AF *)
+  | E_early_data of earlyDataIndication
+  | E_supported_versions of protocol_versions   (* M, AF *) 
+  | E_cookie of b:bytes {0 < length b /\ length b < 65536}  (* M *)
+  | E_psk_key_exchange_modes of client_psk_kexes (* client-only; mandatory when proposing PSKs *)  | E_extended_ms
+  | E_ec_point_format of list ECGroup.point_format
+  | E_unknown_extension of (lbytes 2 * bytes) (* header, payload *)
+(*
+  | E_max_fragment_length
+  | E_status_request
+  | E_use_srtp 
   | E_heartbeat 
   | E_application_layer_protocol_negotiation
   | E_signed_certifcate_timestamp 
   | E_client_certificate_type 
   | E_server_certificate_type 
-  | E_padding *)
-  | E_key_share of CommonDH.keyShare (* M, AF *)
-  | E_pre_shared_key of (list psk) (* M, AF *)
-  | E_early_data of earlyDataIndication
-  | E_supported_versions of protocol_versions   (* M, AF *) 
-  | E_cookie of b:bytes { 1 <= length b /\ length b <= (pow2 16 - 1)}  (* M *)
-  | E_psk_key_exchange_modes of client_psk_kexes (* client-only; mandatory when proposing PSKs *)  
-(*| E_certificate_authorities 
+  | E_certificate_authorities 
   | E_oid_filters 
-  | E_post_handshake_auth *)
-// Previous extension types
-(*| E_renegotiation_info of renegotiationInfo *)
-  | E_extended_ms
-  | E_ec_point_format of list ECGroup.point_format
-  | E_unknown_extension of (lbytes 2 * bytes) (* un-{implemented,known} extensions. *)
-
+  | E_post_handshake_auth 
+  | E_renegotiation_info of renegotiationInfo
+*)
 
 (* string_of_ *)
 let string_of_extension = function
@@ -97,10 +84,9 @@ let string_of_extension = function
   | E_ec_point_format _ -> "ec_point_fmt" 
   | E_unknown_extension (n,_) -> print_bytes n
 
-
 let rec string_of_extensions = function
-  | e0::es -> string_of_extension e0^" "^string_of_extensions es
-  | []  -> ""
+  | e0 :: es -> string_of_extension e0 ^ " " ^ string_of_extensions es
+  | [] -> ""
 
 (** shallow equality *)
 private let sameExt e1 e2 =
@@ -124,7 +110,7 @@ private let sameExt e1 e2 =
  extension formatting
  *************************************************)
  
-private val extensionHeaderBytes: extension -> Tot bytes
+private val extensionHeaderBytes: extension -> lbytes 2
 let extensionHeaderBytes ext =
   match ext with             // 4.2 ExtensionType enum value
   | E_server_name _            -> abyte2 (0x00z, 0x00z)
@@ -138,43 +124,29 @@ let extensionHeaderBytes ext =
   | E_psk_key_exchange_modes _ -> abyte2 (0x00z, 0x2dz) // 45
   | E_extended_ms              -> abyte2 (0x00z, 0x17z) // 45
   | E_ec_point_format _        -> abyte2 (0x00z, 0x0Bz) // 11 
-  | E_unknown_extension(h,b) -> h
+  | E_unknown_extension (h,b)  -> h
 
-private val serverNameBytes: list TI.serverName -> Tot bytes
+private val serverNameBytes: list serverName -> Tot bytes
 let serverNameBytes l =
-    let rec (aux:list TI.serverName -> Tot bytes) = function
-    | [] -> empty_bytes
-    | TI.SNI_DNS(x) :: r -> (abyte 0z) @| bytes_of_int 2 (length x) @| x @| aux r
-    | TI.SNI_UNKNOWN(t, x) :: r -> (bytes_of_int 1 t) @| bytes_of_int 2 (length x) @| x @| aux r
-    in
-    (aux l)
-
-private val extension_depth : extension -> Tot nat
-let rec extension_depth (ext:extension): Tot nat =
-  match ext with
-  | E_early_data edt           -> (
-      match edt with
-      | ServerEarlyDataIndication -> 0
-      | ClientEarlyDataIndication edi -> 1 + extensions_depth edi.ped_extensions
-      )
-  | _ -> 0
-and extensions_depth (exts:list extension): Tot nat =
-  match exts with
-  | [] -> 0
-  | hd::tl -> let x = extensions_depth tl in
-	     let y = extension_depth hd in
-	     if y > x then y else x
-
+  let rec (aux:list serverName -> Tot bytes) = function
+  | [] -> empty_bytes
+  | SNI_DNS(x) :: r -> (abyte 0z) @| bytes_of_int 2 (length x) @| x @| aux r
+  | SNI_UNKNOWN(t, x) :: r -> (bytes_of_int 1 t) @| bytes_of_int 2 (length x) @| x @| aux r
+  in
+  (aux l)
+ 
 val earlyDataIndicationBytes: edi:earlyDataIndication -> Tot bytes
-  (decreases (fun edi -> match edi with | ClientEarlyDataIndication edi -> extensions_depth edi.ped_extensions | _ -> 0))
-val extensionPayloadBytes: role -> ext:extension -> Tot bytes
-  (decreases (extension_depth ext))
+let earlyDataIndicationBytes = function
+  | None -> empty_bytes // ClientHello, EncryptedExtensions
+  | Some max_early_data_size -> // NewSessionTicket
+    let n = UInt32.v max_early_data_size in    
+    lemma_repr_bytes_values n;
+    bytes_of_int 4 n
 
-let rec (ecpfListBytes_aux:list ECGroup.point_format -> Tot bytes) =
-  function
+let rec ecpfListBytes_aux : list ECGroup.point_format -> bytes = function
   | [] -> empty_bytes
   | ECGroup.ECP_UNCOMPRESSED :: r -> (abyte 0z) @| ecpfListBytes_aux r
-  | ECGroup.ECP_UNKNOWN(t) :: r -> (bytes_of_int 1 t) @| ecpfListBytes_aux r
+  | ECGroup.ECP_UNKNOWN t :: r -> (bytes_of_int 1 t) @| ecpfListBytes_aux r
 
 val ecpfListBytes: l:list ECGroup.point_format{length (ecpfListBytes_aux l) < 256} -> Tot bytes
 let ecpfListBytes l =
@@ -182,111 +154,102 @@ let ecpfListBytes l =
   lemma_repr_bytes_values (length al);
   let bl:bytes = vlbytes 1 al in
   bl
-  
-(* API *)
-(** Serialize extension. *)
-val extensionBytes: role -> ext:extension -> Tot bytes
-  (decreases (extension_depth ext))
-val extensionsBytes: role -> cl:list extension -> Tot (b:bytes{length b <= 2 + 65535})
-  (decreases (extensions_depth cl))
 
-let rec earlyDataIndicationBytes edi =
-  match edi with
-  | ServerEarlyDataIndication -> empty_bytes
-  | ClientEarlyDataIndication edi ->
-      let cid_bytes = configurationIdBytes edi.ped_configuration_id in
-      let cs_bytes = cipherSuiteBytes edi.ped_cipher_suite in
-      let ext_bytes = extensionsBytes Client edi.ped_extensions in
-      lemma_repr_bytes_values (length edi.ped_context);
-      let context_bytes = vlbytes 1 edi.ped_context in
-//      let edt_bytes = earlyDataTypeBytes edi.ped_early_data_type in
-      cid_bytes @| cs_bytes @| ext_bytes @| context_bytes //@| edt_bytes
-and extensionPayloadBytes role ext =
-  match ext with
-  | E_server_name(l)           -> 
-      if role = Client then vlbytes 2 (serverNameBytes l) 
-      else serverNameBytes l
-  | E_supported_groups(l)      -> Parse.namedGroupsBytes l  
+(* API *)
+
+// Missing refinements in `extension` type constructors to be able to prove the length bound
+(** Serializes an extension payload *)
+val extensionPayloadBytes: extension -> b:bytes { length b < 65536 - 4 }
+let rec extensionPayloadBytes = function
+  | E_server_name []           -> empty_bytes // ServerHello, EncryptedExtensions
+  | E_server_name l            -> vlbytes 2 (serverNameBytes l) // ClientHello
+  | E_supported_groups l       -> namedGroupsBytes l  
   | E_signature_algorithms sha -> sigHashAlgsBytes sha
   | E_key_share ks             -> CommonDH.keyShareBytes ks
-  | E_pre_shared_key psk -> admit() //PSK.preSharedKeyBytes psk //17-04-21 TODO parse/format the list with ota
-  | E_early_data edt           -> earlyDataIndicationBytes edt
+  | E_pre_shared_key psk       -> admit() //PSK.preSharedKeyBytes psk //17-04-21 TODO parse/format the list with ota
+  | E_early_data edi           -> earlyDataIndicationBytes edi
   | E_supported_versions vv    ->
-      vlbytes 1
-      (List.Tot.fold_left (fun acc v -> acc @| TLSConstants.versionBytes v) empty_bytes vv)
-  | E_cookie c                 -> c // SI: check 
+    // Sending TLS 1.3 draft versions, as other implementations are doing
+    vlbytes 1 (List.Tot.fold_left (fun acc v -> acc @| versionBytes_draft v) empty_bytes vv)
+  | E_cookie c                 -> (lemma_repr_bytes_values (length c); vlbytes 2 c)
   | E_psk_key_exchange_modes _ -> admit()
   | E_extended_ms              -> empty_bytes
   | E_ec_point_format l        -> ecpfListBytes l
-  | E_unknown_extension (h,b)  -> b
-and extensionBytes role ext =
-    let head = extensionHeaderBytes ext in
-    let payload = extensionPayloadBytes role ext in
-    let payload = vlbytes 2 payload in
-    head @| payload
-and extensionsBytes role exts =
-  vlbytes 2 (List.Tot.fold_left (fun l s -> l @| extensionBytes role s) empty_bytes exts)
+  | E_unknown_extension (_,b)  -> b
 
-(* JK: For some reason without that I do not manage to get the
-definition of extensionsBytes *)
-assume val extensionsBytes_def: r:role -> 
-  cl:list extension{repr_bytes (length (List.Tot.fold_left (fun l s -> l @| extensionBytes r s) empty_bytes cl)) <= 2} ->
-  Lemma (requires (True))
-	(ensures (extensionsBytes r cl = vlbytes 2 (List.Tot.fold_left (fun l s -> l @| extensionBytes r s) empty_bytes cl)))
-  [SMTPat (extensionsBytes r cl)]
+(** Serializes an extension *)
+val extensionBytes: ext:extension -> b:bytes { length b < 65536 }
+let rec extensionBytes ext =
+  let head = extensionHeaderBytes ext in
+  let payload = extensionPayloadBytes ext in
+  lemma_repr_bytes_values (length payload);
+  let payload = vlbytes 2 payload in
+  head @| payload
 
-(* TODO: inversion lemmas
-val parseEarlyDataIndication: pinverse_t earlyDataIndicationBytes
-val parseExtension: pinverse_t extensionBytes
-val parseExtensions: pinverse_t extensionsBytes
-*)
+type extensions = 
+  exts:list extension {repr_bytes (length (List.Tot.fold_left (fun l s -> l @| extensionBytes s) empty_bytes exts)) <= 2}
+
+val extensionsBytes: extensions -> b:bytes { length b < 2 + 65536 }
+let extensionsBytes exts =
+  let b = List.Tot.fold_left (fun l s -> l @| extensionBytes s) empty_bytes exts in
+  lemma_repr_bytes_values (length b);
+  vlbytes 2 b
+
+// opaque cert_data<1..2^24-1>
+type cert = b:bytes {length b < 16777216}
+
+// CertificateEntry certificate_list<0..2^24-1>;
+// See https://tlswg.github.io/tls13-spec/#rfc.section.4.4.2
+type chain = l:list (cert * extensions) // { ... }
+
 
 (*************************************************
- extension parsing
- *************************************************)
+ Extension parsing
+**************************************************)
 
 //17-05-01 why not using TLSError.result ?? 
+// SZ: NO idea. We should.
 (** local, failed-to-parse exc. *)
 private type canFail (a:Type) =
 | ExFail of alertDescription * string
 | ExOK of list a
 
-private val parseserverName: r:role -> b:bytes -> Tot (result (list TI.serverName))
+private val parseserverName: r:role -> b:bytes -> result (list serverName)
 let parseserverName r b  =
-  let rec aux: b:bytes -> Tot (canFail TI.serverName) (decreases (length b)) = fun b ->
-    if equalBytes b empty_bytes then ExOK []
+  let rec aux: b:bytes -> Tot (canFail serverName) (decreases (length b)) = fun b ->
+    if length b = 0 then ExOK []
     else if length b >= 3 then
       let ty,v = split b 1 in
       begin
       match vlsplit 2 v with
-      | Error(x,y) ->
-	ExFail(x, "Failed to parse SNI length: "^ (Platform.Bytes.print_bytes b))
-      | Correct(cur, next) ->
+      | Error (x,y) ->
+	ExFail (x, "Failed to parse SNI length: "^ (Platform.Bytes.print_bytes b))
+      | Correct (cur, next) ->
 	begin
 	match aux next with
-	| ExFail(x,y) -> ExFail(x,y)
+	| ExFail z -> ExFail z
 	| ExOK l ->
 	  let cur =
 	    begin
 	    match cbyte ty with
-	    | 0z -> TI.SNI_DNS(cur)
-	    | v  -> TI.SNI_UNKNOWN(int_of_bytes ty, cur)
+	    | 0z -> SNI_DNS cur
+	    | v  -> SNI_UNKNOWN (int_of_bytes ty, cur)
 	    end
 	  in
-	  let snidup: TI.serverName -> Tot bool = fun x ->
+	  let snidup: serverName -> Tot bool = fun x ->
 	    begin
 	    match x,cur with
-	    | TI.SNI_DNS _, TI.SNI_DNS _ -> true
-	    | TI.SNI_UNKNOWN(a,_), TI.SNI_UNKNOWN(b,_) -> a = b
+	    | SNI_DNS _, SNI_DNS _ -> true
+	    | SNI_UNKNOWN (a,_), SNI_UNKNOWN (b,_) -> a = b
 	    | _ -> false
 	    end
 	  in
 	  if List.Tot.existsb snidup l then
 	    ExFail(AD_unrecognized_name, perror __SOURCE_FILE__ __LINE__ "Duplicate SNI type")
-	  else ExOK(cur :: l)
+	  else ExOK (cur :: l)
 	end
       end
-    else ExFail(AD_decode_error, "Failed to parse SNI")
+    else ExFail (AD_decode_error, "Failed to parse SNI")
     in
     match r with
     | Server ->
@@ -299,234 +262,210 @@ let parseserverName r b  =
 	begin
 	match vlparse 2 b with
 	| Error z -> Error(AD_decode_error, perror __SOURCE_FILE__ __LINE__ "Failed to parse SNI list")
-	| Correct b ->
-	match aux b with
-	| ExFail(x,y) -> Error(x,y)
-	| ExOK [] -> Error(AD_unrecognized_name, perror __SOURCE_FILE__ __LINE__ "Empty SNI extension")
-	| ExOK l -> correct l
-	end
+        | Correct b ->
+          match aux b with
+          | ExFail z -> Error z
+          | ExOK [] -> Error (AD_unrecognized_name, perror __SOURCE_FILE__ __LINE__ "Empty SNI extension")
+          | ExOK l -> correct l
+        end
       else
-	Error(AD_decode_error, perror __SOURCE_FILE__ __LINE__ "Failed to parse SNI list")
+        Error (AD_decode_error, perror __SOURCE_FILE__ __LINE__ "Failed to parse SNI list")
 
 private let err_msg s = "Got inapproprite bytes for " ^ s
 
 private val addOnce: extension -> list extension -> Tot (result (list extension))
 let addOnce ext extList =
-    if List.Tot.existsb (sameExt ext) extList then
-        Error(AD_handshake_failure, perror __SOURCE_FILE__ __LINE__ "Same extension received more than once")
-    else
-        let res = FStar.List.Tot.append extList [ext] in
-        correct(res)
+  if List.Tot.existsb (sameExt ext) extList then
+    Error (AD_handshake_failure, perror __SOURCE_FILE__ __LINE__ "Same extension received more than once")
+  else
+    let res = FStar.List.Tot.append extList [ext] in
+    correct res
 
-(* SI: API. Called by HandshakeMessages. *)
-(** Parse extension. *)
-val parseEarlyDataIndication: r:role -> b:bytes -> Tot (result earlyDataIndication) (decreases (length b))
-val parseExtension: r:role -> b:bytes -> Tot (result extension) (decreases (length b))
-val parseExtensions: r:role -> b:bytes -> Tot (result (list extension)) (decreases (length b))
-
-val parseEcpfList: bytes -> Tot (result (list ECGroup.point_format))
+val parseEcpfList: bytes -> result (list ECGroup.point_format)
 let parseEcpfList b =
-    let rec aux:b:bytes -> Tot (canFail (ECGroup.point_format)) (decreases (length b)) = fun b ->
-        if equalBytes b empty_bytes then ExOK([])
-        else
-	  if (0 < length b) then 
-	    let (u,v) = split b 1 in
-              (match aux v with
-              | ExFail(x,y) -> ExFail(x,y)
-              | ExOK(l) ->
-                  let cur = match cbyte u with
-                  | 0z -> ECGroup.ECP_UNCOMPRESSED
-                  | _ -> ECGroup.ECP_UNKNOWN(int_of_bytes u)
-                  in ExOK(cur :: l))
-	  else ExFail(AD_decode_error, perror __SOURCE_FILE__ __LINE__ "Malformed curve list")
-    in match aux b with
-    | ExFail(x,y) -> Error(x,y)
-    | ExOK(l) -> 
-      if (List.Tot.mem ECGroup.ECP_UNCOMPRESSED l) then
-	correct l
-      else
-        Error(AD_decode_error, perror __SOURCE_FILE__ __LINE__ "Uncompressed point format not supported")
+  let rec aux:b:bytes -> Tot (canFail (ECGroup.point_format)) (decreases (length b)) = fun b ->
+    if equalBytes b empty_bytes then ExOK []
+    else
+      if 0 < length b then 
+        let u, v = split b 1 in
+        begin
+	match aux v with
+	| ExFail (x, y) -> ExFail (x, y)
+	| ExOK l ->
+	  let cur = 
+            match cbyte u with
+	    | 0z -> ECGroup.ECP_UNCOMPRESSED
+	    | _  -> ECGroup.ECP_UNKNOWN (int_of_bytes u)
+	  in ExOK (cur :: l)
+        end
+      else ExFail (AD_decode_error, perror __SOURCE_FILE__ __LINE__ "Malformed curve list")
+  in
+  match aux b with
+  | ExFail z -> Error z
+  | ExOK l -> 
+    if List.Tot.mem ECGroup.ECP_UNCOMPRESSED l then
+      correct l
+    else
+      Error (AD_decode_error, perror __SOURCE_FILE__ __LINE__ "Uncompressed point format not supported")
 
-(* We don't care about duplicates, not formally excluded. *)
- 
+
 //17-05-01 added a refinement to control the list length; this function verifies.
 //17-05-01 should we use generic code to parse such bounded lists?
+//REMARK: We don't care about duplicates, not formally excluded.
 //REMARK: This is not tail recursive, contrary to most of our parsing functions
 val parseVersions: 
   b:bytes -> 
-  Tot (result (l:list TLSConstants.protocolVersion {FStar.Mul.( length b == 2 * List.Tot.length l)})) (decreases (length b))
+  Tot (result (l:list protocolVersion {length b == FStar.Mul.(2 * List.Tot.length l)}))
+      (decreases (length b))
 let rec parseVersions b =
   match length b with 
   | 0 -> let r = [] in assert_norm (List.Tot.length [] = 0); Correct r
-  | 1 -> Error (AD_decode_error, "malformed version list") 
+  | 1 -> Error (AD_decode_error, "malformed version list")
   | _ -> 
     let b2, b' = split b 2 in
-    match TLSConstants.parseVersion b2 with 
+    match parseVersion_draft b2 with
     | Error z -> Error z
     | Correct v -> 
       match parseVersions b' with 
       | Error z -> Error z 
-      | Correct vs -> (
-          let r = v::vs in 
-          assert_norm (List.Tot.length (v::vs) = 1 + List.Tot.length vs); // did not find usable length lemma in List.Tot
-          Correct r)
-
-let parseSupportedVersions (b:bytes) : result (list TLSConstants.protocolVersion) =
+      | Correct vs ->
+        begin
+ 	let r = v::vs in 
+	assert_norm (List.Tot.length (v::vs) = 1 + List.Tot.length vs); // did not find usable length lemma in List.Tot
+	Correct r
+        end
+  
+val parseSupportedVersions: b:bytes{2 < length b /\ length b < 256} -> result protocol_versions
+let parseSupportedVersions b =
   match vlparse 1 b with
   | Correct b ->
     begin
-    match parseVersions b with
-    | Correct pvs ->
-      let n = List.Tot.length pvs in
-      if 1 <= n && n <= 127 then Correct pvs else
-      Error(AD_decode_error, perror __SOURCE_FILE__ __LINE__ "Too many or too few protocol versions")
+    match parseVersions b with // Necessary for verification
+    | Correct l -> Correct l
     | Error z -> Error z
     end
-  | Error z ->
-    Error(AD_decode_error, perror __SOURCE_FILE__ __LINE__ "Failed to parse protocol versions")
+  | Error z -> Error z
 
+val parseEarlyDataIndication: b:bytes{length b == 0 \/ length b == 4} -> earlyDataIndication
+let parseEarlyDataIndication b =
+  if length b = 0 then None
+  else
+    begin
+    let n = int_of_bytes b in
+    lemma_repr_bytes_values n;
+    assert_norm (pow2 32 == 4294967296);
+    Some (UInt32.uint_to_t n)
+    end
+
+val parseExtension: role -> b:bytes -> result extension
 let rec parseExtension role b =
-  if length b >= 4 then
-    let (head, payload) = split b 2 in
+  if length b < 4 then
+    Error (AD_decode_error, perror __SOURCE_FILE__ __LINE__ "Extension bytes are too short to store even the extension type")
+  else
+    let head, payload = split b 2 in
     match vlparse 2 payload with
-    | Correct (data) ->
-	(match cbyte2 head with
+    | Error _ -> 
+      Error(AD_decode_error, perror __SOURCE_FILE__ __LINE__ "Failed to parse extension length 1")
+    | Correct data ->
+      begin
+      match cbyte2 head with
+      | (0x00z, 0x00z) -> // SNI
+        mapResult E_server_name (parseserverName role data)
+      | (0x00z, 0x0Az) -> // supported groups
+        if 2 <= length data && length data < 65538 then
+         (match parseNamedGroups data with
+          | Correct l -> Correct (E_supported_groups l)
+          | Error z -> Error z)
+        else Error (AD_decode_error, perror __SOURCE_FILE__ __LINE__ (err_msg "SNI"))
+      | (0x00z, 0x0Dz) -> // sigAlgs
+        if 2 <= length data && length data < 65538 then
+          (match parseSigHashAlgs data with
+           | Correct algs -> Correct (E_signature_algorithms algs)
+           | Error z -> Error z)
+        else Error (AD_decode_error, perror __SOURCE_FILE__ __LINE__ (err_msg "sigAlgs"))
+      | (0x00z, 0x28z) -> // keyShare
+        (match CommonDH.parseKeyShare (Client? role) data with
+         | Correct ks -> Correct (E_key_share ks)
+         | Error z -> Error z)
+      | (0x00z, 0x29z) -> // head TBD, PSK
+        if length data >= 2 then
+          (match admit() (* 17-04-21 TODO PSK.parsePreSharedKey data *) with
+           | Correct psk -> Correct psk
+           | Error z -> Error z)
+        else Error (AD_decode_error, perror __SOURCE_FILE__ __LINE__ (err_msg "PSK"))
+      | (0x00z, 0x2az) -> // EDI
+        if length data = 0 || length data = 4 then
+          (match parseEarlyDataIndication data with
+           | None -> Correct (E_early_data None)
+           | Some n -> Correct (E_early_data (Some n)))
+        else Error (AD_decode_error, perror __SOURCE_FILE__ __LINE__ (err_msg "early_data")) 
+      | (0x00z, 0x2bz) -> // supported_versions
+        if 2 < length data && length data < 256 then
+          (match parseSupportedVersions data with
+           | Correct v -> Correct (E_supported_versions v)
+           | Error z -> Error z)
+        else Error (AD_decode_error, perror __SOURCE_FILE__ __LINE__ (err_msg "supported_versions"))
+      | (0xffz, 0x2cz) -> // cookie
+        if 0 < length data && length data < 65536 then
+	  Correct (E_cookie data)
+	else Error(AD_decode_error, perror __SOURCE_FILE__ __LINE__ (err_msg "cookie"))
+(* ToDo: | E_psk_key_exchange_modes _ *)
 (*
-        | (0xffz, 0x02z) -> // TLS 1.3 draft version
-          if length data = 2 then Correct (E_draftVersion data)
-          else Error (AD_decode_error, perror __SOURCE_FILE__ __LINE__ (err_msg "draft 1.3 version"))
-
-*)	
-	| (0x00z, 0x00z) -> // sni
-	  (match parseserverName role data with
-	  | Correct(snis) -> Correct (E_server_name snis)
-	  | Error(z) -> Error(z))	  
-	| (0x00z, 0x0Az) -> // supported groups
-	  if length data >= 2 && length data < 65538 then
-	  (match Parse.parseNamedGroups (data) with
-	  | Correct(groups) -> Correct (E_supported_groups(groups))
-	  | Error(z) -> Error(z))
-	  else Error (AD_decode_error, perror __SOURCE_FILE__ __LINE__ (err_msg "SNI"))
-	| (0x00z, 0x0Dz) -> // sigAlgs
-	  if length data >= 2 && length data < 65538 then (
-	  (match TLSConstants.parseSigHashAlgs data with
-	  | Correct(algs) -> Correct (E_signature_algorithms algs)
-	  | Error(z) -> Error(z))
-	  ) else Error (AD_decode_error, perror __SOURCE_FILE__ __LINE__ (err_msg "sigAlgs"))
-	| (0x00z, 0x28z) -> // keyShare
-	  (let is_client = (match role with | Client -> true | Server -> false) in
-	  match CommonDH.parseKeyShare is_client data with
-	  | Correct (ks) -> Correct (E_key_share(ks))
-	  | Error(z) -> Error(z))
-	| (0x00z, 0x29z) -> // head TBD, PSK
-	  if length data >= 2 then
-	  (match admit() (* 17-04-21 TODO PSK.parsePreSharedKey data *) with
-	  | Correct(psk) -> Correct (E_pre_shared_key psk)
-	  | Error(z) -> Error(z))
-	  else Error (AD_decode_error, perror __SOURCE_FILE__ __LINE__ (err_msg "PSK"))
-	| (0x00z, 0x2az) -> // EDI
-	  (match parseEarlyDataIndication role data with
-	  | Correct (edi) -> Correct (E_early_data(edi))
-	  | Error(z) -> Error(z))
-        | (0x00z, 0x2bz) -> // supported_versions
-	  (match parseSupportedVersions data with
-	  | Correct v -> Correct (E_supported_versions v)
-	  | Error z -> Error z)
-        | (0xffz, 0x2cz) -> // cookie
-	  if length data >= 1 && length data <= ((pow2 16) - 1) then 
-	    Correct (E_cookie data)
-	  else Error(AD_decode_error, perror __SOURCE_FILE__ __LINE__ (err_msg "cookie"))
-        (* ToDo: | E_psk_key_exchange_modes _ *)
-(*
-        | (0xffz, 0x02z) -> // TLS 1.3 draft version
-          if length data = 2 then Correct (E_draftVersion data)
-          else Error (AD_decode_error, perror __SOURCE_FILE__ __LINE__ "Got inappropriate draft 1.3 version")
 	| (0xFFz, 0x01z) -> // renego (* OLD *)
 	  (match parseRenegotiationInfo data with
 	  | Correct(ri) -> Correct (E_renegotiation_info(ri))
-	  | Error(z) -> Error(z)
+	  | Error z -> Error z
 *)	 
 	| (0x00z, 0x17z) -> // extended ms
 	  if length data = 0 then Correct (E_extended_ms)
 	  else Error (AD_decode_error, perror __SOURCE_FILE__ __LINE__ "Got inappropriate bytes for extended MS extension")
 	| (0x00z, 0x0Bz) -> // ec point format
-	  if length data < 256 && length data >= 1 then
-	  (lemma_repr_bytes_values (length data);
-	  match vlparse 1 data with
-	  | Error(z) -> Error(z)
-	  | Correct(data) ->
-	  match parseEcpfList data with
-	  | Correct(ecpfs) -> Correct (E_ec_point_format(ecpfs))
-	  | Error(z) -> Error(z))
+	  if 1 <= length data && length data < 256 then
+	    (lemma_repr_bytes_values (length data);
+	     match vlparse 1 data with
+	     | Error z -> Error z
+	     | Correct data ->
+	       match parseEcpfList data with
+	       | Correct ecpfs -> Correct (E_ec_point_format ecpfs)
+	       | Error z -> Error z)
 	  else Error (AD_decode_error, perror __SOURCE_FILE__ __LINE__ (err_msg "ec_point_fmt"))
 	| _ -> // Unknown extension
-	  Correct(E_unknown_extension(head,data)))
-    | Error(z) -> Error(AD_decode_error, perror __SOURCE_FILE__ __LINE__ "Failed to parse extension length 1")
-  else Error (AD_decode_error, perror __SOURCE_FILE__ __LINE__ "Extension bytes are too short to store even the extension type")
-and parseEarlyDataIndication role b =
-  if length b >= 2 then
-    match vlsplit 2 b with
-    | Correct(config_id, data) ->
-      if length config_id > 2 then (
-      lemma_repr_bytes_values (length config_id);
-      match parseConfigurationId (vlbytes 2 config_id) with
-      | Correct(cid) -> (
-	if length data >= 2 then
-	  let (cs, data) = split data 2 in
-	  match parseCipherSuite cs with
-	  | Correct(cs) ->
-	    if length data >= 2 then (
-	    match vlsplit 2 data with
-	    | Correct(exts, data) -> (
-	      match parseExtensions role (vlbytes 2 exts) with
-	      | Correct(exts) ->
-		if length data >= 1 then (
-		match vlparse 1 data with
-		| Correct(ctx) ->
-		    Correct (ClientEarlyDataIndication ({ ped_configuration_id = cid;
-							  ped_cipher_suite = cs;
-							  ped_extensions = exts;
-							  ped_context = ctx; }))
-		| Error(z) -> Error(z) )
-		else Error (AD_decode_error, perror __SOURCE_FILE__ __LINE__ "Not enough bytes to parse cipher suite in early data indication")
-	      | Error(z) -> Error(z) )
-	    | Error(z) -> Error(z) )
-	    else Error (AD_decode_error, perror __SOURCE_FILE__ __LINE__ "Not enough bytes to parse cipher suite in early data indication")
-	  | Error(z) -> Error(z)
-	else Error (AD_decode_error, perror __SOURCE_FILE__ __LINE__ "Not enough bytes to parse cipher suite in early data indication") )
-      | Error(z) -> Error(z) )
-      else Error (AD_decode_error, perror __SOURCE_FILE__ __LINE__ "Got inappropriate bytes for configuration id")
-    | Error(z) -> Error(AD_decode_error, perror __SOURCE_FILE__ __LINE__ "Failed to parse early data indication length")
-  else Correct (ServerEarlyDataIndication)
-and parseExtensions role b =
-  let rec (aux:bytes -> list extension -> Tot (result (list extension))) = fun b exts ->
+          Correct (E_unknown_extension (head,data))
+        end
+
+val parseExtensions: role -> b:bytes -> result (list extension)
+let rec parseExtensions role b =
+  let rec aux: 
+    b:bytes -> list extension -> Tot (result (list extension)) (decreases (length b)) = fun b exts ->
     if length b >= 4 then
       let ht, b = split b 2 in
       match vlsplit 2 b with
-      | Correct(ext, bytes) -> (
-	(* assume (Prims.precedes (Prims.LexCons b) (Prims.LexCons (ht @| vlbytes 2 ext))); *)
+      | Correct (ext, bytes) ->
+        begin
 	match parseExtension role (ht @| vlbytes 2 ext) with
-	| Correct(ext) ->
-	  (match addOnce ext exts with // fails if the extension already is in the list
-	  | Correct(exts) -> aux bytes exts
-	  | Error(z) -> Error(z))
-	| Error(z) -> Error(z))
-      | Error(z) -> Error(AD_decode_error, perror __SOURCE_FILE__ __LINE__ "Failed to parse extension length 2")
-    else Correct(exts) in
+	| Correct ext ->
+          begin
+	  match addOnce ext exts with // fails if the extension already is in the list
+	  | Correct exts -> aux bytes exts
+	  | Error z -> Error z
+          end
+	| Error z -> Error z
+        end
+      | Error z -> Error (AD_decode_error, perror __SOURCE_FILE__ __LINE__ "Failed to parse extension length 2")
+    else Correct exts in
   if length b >= 2 then
-  match vlparse 2 b with
-  | Correct(b) -> aux b []
-  | Error(z) -> Error(AD_decode_error, perror __SOURCE_FILE__ __LINE__ "Failed to parse extensions length")
-  else Error(AD_decode_error, perror __SOURCE_FILE__ __LINE__ "Failed to parse extensions length")
+    match vlparse 2 b with
+    | Correct b -> aux b []
+    | Error z -> 
+      Error(AD_decode_error, perror __SOURCE_FILE__ __LINE__ "Incorrect extension data length")
+  else 
+    Error(AD_decode_error, perror __SOURCE_FILE__ __LINE__ "Failed to parse extensions length")
 
 (* SI: API. Called by HandshakeMessages. *)
-val parseOptExtensions: r:role -> data:bytes -> Tot (result (option (list extension)))
+val parseOptExtensions: r:role -> data:bytes -> result (option (list extension))
 let parseOptExtensions r data =
-  if length data = 0 then Correct(None)
-  else
-  (match parseExtensions r data with
-  | Correct(exts) -> Correct(Some exts)
-  | Error(z) -> Error(z))
+  if length data = 0 then Correct None
+  else mapResult Some (parseExtensions r data)
 
 
 (*************************************************
@@ -535,12 +474,12 @@ let parseOptExtensions r data =
 
 (* JK: Need to get rid of such functions *)
 (* API. Called by Negotiation *)
-let rec list_valid_cs_is_list_cs (l:valid_cipher_suites): Tot (list cipherSuite) =
+let rec list_valid_cs_is_list_cs (l:valid_cipher_suites): list cipherSuite =
   match l with 
   | [] -> [] 
   | hd :: tl -> hd :: list_valid_cs_is_list_cs tl
   
-private let rec list_valid_ng_is_list_ng (#p:(namedGroup -> Type)) (l:list (n:namedGroup{p n})): Tot (list namedGroup) = 
+private let rec list_valid_ng_is_list_ng (#p:namedGroup -> Type) (l:list (n:namedGroup{p n})) : list namedGroup = 
   match l with 
   | [] -> [] 
   | hd :: tl -> hd :: list_valid_ng_is_list_ng tl
@@ -569,9 +508,9 @@ val prepareExtensions:
   bool -> 
   bool -> 
   list sigHashAlg -> list (x:namedGroup{SEC? x \/ FFDHE? x}) -> 
-  option (TI.cVerifyData * TI.sVerifyData) -> 
+  option (cVerifyData * sVerifyData) ->
   option CommonDH.keyShare -> 
-  Tot (l:list extension{List.Tot.length l < 256})
+  l:list extension{List.Tot.length l < 256}
 (* SI: implement this using prep combinators, of type exts->data->exts, per ext group. 
    For instance, PSK, HS, etc extensions should all be done in one function each. 
    This seems to make this prepareExtensions more modular. *)
@@ -623,7 +562,7 @@ val matchExtensions: list extension{List.Tot.length l < 256} -> Tot (
   bool *
   bool * 
   list sigHashAlg -> list (x:namedGroup{SEC? x \/ FFDHE? x}) *
-  option (TI.cVerifyData * TI.sVerifyData) *
+  option (cVerifyData * sVerifyData) *
   option CommonDH.keyShare )
 let matchExtensions ext = admit()
 
@@ -644,8 +583,8 @@ let prepareExtensions_inverse pv cs sres sren sigAlgs namedGroups ri ks:
 (*
 type renegotiationInfo =
   | FirstConnection
-  | ClientRenegotiationInfo of (TI.cVerifyData)
-  | ServerRenegotiationInfo of (TI.cVerifyData * TI.sVerifyData)
+  | ClientRenegotiationInfo of (cVerifyData)
+  | ServerRenegotiationInfo of (cVerifyData * sVerifyData)
 
 val renegotiationInfoBytes: renegotiationInfo -> Tot bytes
 let renegotiationInfoBytes ri =
@@ -676,13 +615,13 @@ let parseRenegotiationInfo b =
 	    let cvd, svd = split payload 36 in
 	    Correct (ServerRenegotiationInfo (cvd, svd))
 	| _ -> Error (AD_decode_error, perror __SOURCE_FILE__ __LINE__ "Inappropriate length for renegotiation info data (expected 12/24 for client/server in TLS1.x, 36/72 for SSL3"))
-    | Error(z) -> Error(AD_decode_error, perror __SOURCE_FILE__ __LINE__ "Failed to parse renegotiation info length")
+    | Error z -> Error(AD_decode_error, perror __SOURCE_FILE__ __LINE__ "Failed to parse renegotiation info length")
   else Error (AD_decode_error, perror __SOURCE_FILE__ __LINE__ "Renegotiation info bytes are too short")
 *)
 
 (* TODO: remove *)
-private val replace_subtyping: (o:(option (TI.cVerifyData * TI.sVerifyData))) -> Tot (option (bytes*bytes)) 
-let replace_subtyping (o:(option (TI.cVerifyData * TI.sVerifyData))) : Tot (option (bytes*bytes)) =
+private val replace_subtyping: (o:(option (cVerifyData * sVerifyData))) -> Tot (option (bytes*bytes))
+let replace_subtyping (o:(option (cVerifyData * sVerifyData))) : Tot (option (bytes*bytes)) =
   match o with
   | None -> None
   | Some (a,b) -> Some (a,b)
@@ -690,8 +629,8 @@ let replace_subtyping (o:(option (TI.cVerifyData * TI.sVerifyData))) : Tot (opti
 // TODO
 // ADL the negotiation of renegotiation indication is incorrect
 // ADL needs to be consistent with clientToNegotiatedExtension
-private val serverToNegotiatedExtension: TI.config -> list extension -> cipherSuite -> option (TI.cVerifyData * TI.sVerifyData) -> bool -> result TI.negotiatedExtensions -> extension -> Tot (result (TI.negotiatedExtensions))
-let serverToNegotiatedExtension cfg cExtL cs ri (resuming:bool) res sExt : result (TI.negotiatedExtensions)=
+private val serverToNegotiatedExtension: config -> list extension -> cipherSuite -> option (cVerifyData * sVerifyData) -> bool -> result negotiatedExtensions -> extension -> Tot (result (negotiatedExtensions))
+let serverToNegotiatedExtension cfg cExtL cs ri (resuming:bool) res sExt : result (negotiatedExtensions)=
     match res with
     | Error(x,y) -> Error(x,y)
     | Correct(l) ->
@@ -714,42 +653,41 @@ let serverToNegotiatedExtension cfg cExtL cs ri (resuming:bool) res sExt : resul
             correct(l)
 	  else
             Error(AD_handshake_failure,perror __SOURCE_FILE__ __LINE__ "Server sent an SNI acknowledgement without an SNI provided")
-      | E_extended_ms -> correct ({l with TI.ne_extended_ms = true})
+      | E_extended_ms -> correct ({l with ne_extended_ms = true})
       | E_ec_point_format spf ->
 	  if resuming then
             correct l
           else
-            correct ({l with TI.ne_supported_point_formats = Some spf})
+            correct ({l with ne_supported_point_formats = Some spf})
 (* not allowed for server
       | E_signature_algorithms sha ->
           if resuming then correct l
 	  else correct ({l with ne_signature_algorithms = Some (sha)})
 *)
       | E_key_share (CommonDH.ServerKeyShare sks) ->
-        Correct ({l with TI.ne_keyShare = Some sks})
+        Correct ({l with ne_keyShare = Some sks})
       | E_supported_groups named_group_list ->
-        Correct ({l with TI.ne_supported_groups = Some named_group_list})
+        Correct ({l with ne_supported_groups = Some named_group_list})
       | _ -> Error (AD_handshake_failure,perror __SOURCE_FILE__ __LINE__ "Unexpected pattern in serverToNegotiatedExtension")
      else
        Error(AD_handshake_failure,perror __SOURCE_FILE__ __LINE__ "Server sent an extension not present in client hello")
 
 
 (* SI: API. Called by Negotiation. *)
-val negotiateClientExtensions: protocolVersion -> TI.config -> option (list extension) -> option (list extension) -> cipherSuite -> option (TI.cVerifyData * TI.sVerifyData) -> bool -> Tot (result (TI.negotiatedExtensions))
+val negotiateClientExtensions: protocolVersion -> config -> option (list extension) -> option (list extension) -> cipherSuite -> option (cVerifyData * sVerifyData) -> bool -> Tot (result (negotiatedExtensions))
 let negotiateClientExtensions pv cfg cExtL sExtL cs ri (resuming:bool) =
   match pv with
   | SSL_3p0 ->
      begin
      match sExtL with
-     | None -> Correct TI.ne_default
+     | None -> Correct ne_default
      | _ -> Error(AD_internal_error, perror __SOURCE_FILE__ __LINE__ "Received extensions in SSL 3.0 server hello")
      end
   | _ ->
      begin 
      match cExtL, sExtL with
-     | _, None when pv <> TLS_1p3 -> Correct TI.ne_default
      | Some cExtL, Some sExtL -> (
-        let nes = TI.ne_default in
+        let nes = ne_default in
         match List.Tot.fold_left (serverToNegotiatedExtension cfg cExtL cs ri resuming) (correct nes) sExtL with
         | Error(x,y) -> Error(x,y)
         | Correct l ->
@@ -758,37 +696,39 @@ let negotiateClientExtensions pv cfg cExtL sExtL cs ri (resuming:bool) =
 	  begin
 	    match List.Tot.tryFind E_signature_algorithms? cExtL with
 	    | Some (E_signature_algorithms shal) ->
-	      correct({l with TI.ne_signature_algorithms = Some shal})
+	      correct({l with ne_signature_algorithms = Some shal})
 	    | None -> correct l
 	    | _ -> Error(AD_internal_error, perror __SOURCE_FILE__ __LINE__ "Unappropriate sig algs in negotiateClientExtensions")
 	  end )
+     | _, None -> 
+       if pv <> TLS_1p3 then Correct ne_default
+       else Error(AD_internal_error, perror __SOURCE_FILE__ __LINE__ "negoClientExts missing extensions in TLS hello message")
      | _ -> Error(AD_internal_error, perror __SOURCE_FILE__ __LINE__ "negoClientExts missing extensions in TLS hello message")
      end 
-
+     
 (* SI: API. Called by Negotiation. *)
-val clientToNegotiatedExtension: TI.config -> cipherSuite -> option (TI.cVerifyData * TI.sVerifyData) -> bool -> TI.negotiatedExtensions -> extension -> Tot TI.negotiatedExtensions
-let clientToNegotiatedExtension (cfg:TI.config) cs ri resuming neg cExt =
+val clientToNegotiatedExtension: config -> cipherSuite -> option (cVerifyData * sVerifyData) -> bool -> negotiatedExtensions -> extension -> Tot negotiatedExtensions
+let clientToNegotiatedExtension (cfg:config) cs ri resuming neg cExt =
   match cExt with
   | E_supported_groups l ->
       if resuming then neg
       else
-	  let isOK g = List.Tot.existsb (fun (x:Parse.namedGroup) -> x = g) (list_valid_ng_is_list_ng cfg.TI.namedGroups) in
-	  {neg with TI.ne_supported_groups = Some (List.Tot.filter isOK l)}
-
+	  let isOK g = List.Tot.existsb (fun (x:Parse.namedGroup) -> x = g) (list_valid_ng_is_list_ng cfg.namedGroups) in
+	  {neg with ne_supported_groups = Some (List.Tot.filter isOK l)}
   | E_ec_point_format l ->
       if resuming then neg
       else
 	  let nl = List.Tot.filter (fun x -> x = ECGroup.ECP_UNCOMPRESSED) l in
-	  {neg with TI.ne_supported_point_formats = Some nl}
+	  {neg with ne_supported_point_formats = Some nl}
   | E_server_name l ->
-      {neg with TI.ne_server_names = Some l}
+      {neg with ne_server_names = Some l}
   | E_signature_algorithms sha ->
       if resuming then neg
-      else {neg with TI.ne_signature_algorithms = Some (sha)}
+      else {neg with ne_signature_algorithms = Some (sha)}
   | _ -> neg // TODO: handle all remaining cases
 
 
-private val clientToServerExtension: protocolVersion -> TI.config -> cipherSuite -> option (TI.cVerifyData * TI.sVerifyData) -> option CommonDH.keyShare -> bool -> extension -> option extension
+private val clientToServerExtension: protocolVersion -> config -> cipherSuite -> option (cVerifyData * sVerifyData) -> option CommonDH.keyShare -> bool -> extension -> option extension
 let clientToServerExtension pv cfg cs ri ks resuming cext =
   match cext with
   | E_key_share _ ->
@@ -796,7 +736,7 @@ let clientToServerExtension pv cfg cs ri ks resuming cext =
   | E_server_name server_name_list ->
     begin
     // See https://tools.ietf.org/html/rfc6066
-    match pv, List.Tot.tryFind TI.SNI_DNS? server_name_list with
+    match pv, List.Tot.tryFind SNI_DNS? server_name_list with
     | TLS_1p3, _   -> None // TODO: SNI goes in EncryptedExtensions in TLS 1.3
     | _, Some name -> Some (E_server_name [])
     end
@@ -807,7 +747,7 @@ let clientToServerExtension pv cfg cs ri ks resuming cext =
     else
       Some (E_ec_point_format [ECGroup.ECP_UNCOMPRESSED])
   | E_supported_groups named_group_list ->
-    Some (E_supported_groups cfg.TI.namedGroups) // Purely informative
+    Some (E_supported_groups cfg.namedGroups) // Purely informative
   // TODO: handle all remaining cases
   | E_early_data b -> None
   | E_pre_shared_key b -> None
@@ -815,7 +755,7 @@ let clientToServerExtension pv cfg cs ri ks resuming cext =
 
 
 (* SI: API. Called by Handshake. *)
-val negotiateServerExtensions: protocolVersion -> option (list extension) -> valid_cipher_suites -> TI.config -> cipherSuite -> option (TI.cVerifyData*TI.sVerifyData) -> option CommonDH.keyShare -> bool -> Tot (result (option (list extension)))
+val negotiateServerExtensions: protocolVersion -> option (list extension) -> valid_cipher_suites -> config -> cipherSuite -> option (cVerifyData*sVerifyData) -> option CommonDH.keyShare -> bool -> Tot (result (option (list extension)))
 let negotiateServerExtensions pv cExtL csl cfg cs ri ks resuming =
    match cExtL with
    | Some cExtL ->
@@ -841,7 +781,8 @@ let default_sigHashAlg_fromSig pv sigAlg=
     | RSASIG ->
         (match pv with
         | TLS_1p2 -> [(RSASIG, Hash SHA1)]
-        | TLS_1p0 | TLS_1p1 | SSL_3p0 -> [(RSASIG,MD5SHA1)])
+        | TLS_1p0 | TLS_1p1 | SSL_3p0 -> [(RSASIG,MD5SHA1)]
+        | TLS_1p3 -> unexpected "[default_sigHashAlg_fromSig] invoked on TLS 1.3")
         //| SSL_3p0 -> [(RSASIG,NULL)]
     | DSA ->
         [(DSA,Hash SHA1)]
@@ -853,8 +794,7 @@ let default_sigHashAlg_fromSig pv sigAlg=
 (* SI: API. Called by HandshakeMessages. *)
 val default_sigHashAlg: protocolVersion -> cipherSuite -> ML (l:list sigHashAlg{List.Tot.length l <= 1})
 let default_sigHashAlg pv cs =
-    default_sigHashAlg_fromSig pv (sigAlg_of_ciphersuite cs)
-
+  default_sigHashAlg_fromSig pv (sigAlg_of_ciphersuite cs)
 
 
 (*
@@ -940,32 +880,6 @@ let rec cert_type_list_to_SigAlg ctl =
     | [] -> []
     | h::t -> (cert_type_to_SigAlg h) :: (cert_type_list_to_SigAlg t)
 *)
-// JK : cannot add total effect here because of the exception thrown
-(* JK: changed from Tot (list sigHashAlg) to Tot (result (list (sigAlg*hashAlg))) to match the
-   spec to the code *)
-(* val default_sigHashAlg_fromSig: protocolVersion -> sigAlg -> Tot (result (list (sigAlg*hashAlg))) *)
-(* let default_sigHashAlg_fromSig pv sigAlg= *)
-(*     match sigAlg with *)
-(*     | RSASIG -> ( *)
-(*         match pv with *)
-(*         | TLS_1p2 -> Correct [(RSASIG, Hash SHA1)] *)
-(*         | TLS_1p0 | TLS_1p1 | SSL_3p0 -> Correct [(RSASIG,MD5SHA1)] *)
-(* 	| _ -> Error (AD_internal_error, perror __SOURCE_FILE__ __LINE__ "[default_sigHashAlg_fromSig] invoked on an invalid") *)
-(* 	) *)
-(*         //| SSL_3p0 -> [(RSASIG,NULL)] *)
-(*     | DSA -> *)
-(*         Correct [(DSA,Hash SHA1)] *)
-(*         //match pv with *)
-(*         //| TLS_1p0| TLS_1p1 | TLS_1p2 -> [(DSA, SHA1)] *)
-(*         //| SSL_3p0 -> [(DSA,NULL)] *)
-(*     | _ -> Error(AD_internal_error, perror __SOURCE_FILE__ __LINE__ "[default_sigHashAlg_fromSig] invoked on an invalid signature algorithm") *)
-
-(* val default_sigHashAlg: protocolVersion -> cipherSuite -> (result (l:list sigHashAlg{List.Tot.length l <= 1})) *)
-(* let default_sigHashAlg pv cs = *)
-(*   admit(); *)
-(*   match default_sigHashAlg_fromSig pv (sigAlg_of_ciphersuite cs) with *)
-(*   | Correct (l) -> Correct(l) *)
-(*   | Error(z) -> Error(z) *)
 
 (* val sigHashAlg_contains: list sigHashAlg -> sigHashAlg -> Tot bool *)
 (* let sigHashAlg_contains (algList:list sigHashAlg) (alg:sigHashAlg) = *)
